## Formulas

### Difference of Squares

https://www.storyofmathematics.com/difference-of-squares/

$a^2 ‚Äì b^2 = (a + b) (a ‚Äì b)$

### Perfect Square Trinomial

https://www.storyofmathematics.com/perfect-square-trinomial/

$(a+b)(a+b)=a^2+2ab+b^2$

$(a-b)(a-b)=a^2-2ab+b^2$

$(a \pm b)^2=a^2 \pm 2ab+b^2$

## Expressions and equations

### Expressions vs. Equations

An expression is a combination of variables and numbers that undergo operations such as addition, subtraction, multiplication, division, and more.  
Below are some examples of expressions:
- x + 5
- x - 12
- 7 √ó 4x - x2
- $\frac{x}{3}$
- (x2)(x + 4)

<br/><br/>

Equations on the other hand, have a relationship. Often it is a relationship between two expressions separated by some kind of symbol, be it an equals sign (=), inequality symbol (<, >, ‚â•), or some other symbol.  
$x - 4 = 12 - 3x$  
$x + 3x = 12 + 4$  
$4x = 16$  
$x = 4$  

### Equality

### Substitution

## Radical

A radical expression, also referred to as an $n^{th}$ root, or simply radical, is an expression that involves a root.

Radicals are expressed using a radicand (similar to a dividend), a radical symbol, and an index, which is typically denoted as "n."

a radical written without an index is assumed to be a square root.

![alt](https://www.math.net/img/a/algebra/radical/radical/radical.svg)

The above figure, as a whole, makes up a radical. It is read as "the $n^{th}$ root of (x + 2)."

Note that radicals and exponents are closely related, and a radical can be written as the radicand raised to the power of $\frac{1}{n}$

$$\sqrt[n]{x}=x^{\frac{1}{n}}$$

### Properties of radicals

$\sqrt[n]{xy}$ = $\sqrt[n]{x}\times\sqrt[n]{y}$

$\sqrt[n]{\frac{x}{y}}$ = $\frac{\sqrt[n]{x}}{\sqrt[n]{y}}$

---

if $\;x^n=z\;$ then $\;x=\sqrt[n]{z}\;$; z must be ‚â• 0 for even n)  
Example: $\;10^2=100$; $10=\sqrt[2]{100}$



$\sqrt[n]{x^n}=x$; (if x ‚â• 0 or if n is odd)


$\sqrt[n]{x^n}=|x|$; (when x < 0 and n is even)


$\sqrt[n]{x^m}=(\sqrt[n]{x})^m$

### Simplifying radicals
 
Simplifying square root radicals involves using the following property of radicals:  
$\sqrt{xy}=\sqrt{x} \times \sqrt{y}$

$\sqrt{44}=\sqrt{4} \times \sqrt{11}=2\sqrt{11}$

$\sqrt{96}=\sqrt{16} \times \sqrt{6}=4\sqrt{6}$

$\sqrt{\frac{5}{9}}=\sqrt{\frac{1}{9}} \times \sqrt{5}=\frac{1}{3}\sqrt{5}$ OR $\sqrt{\frac{5}{9}}=\frac{\sqrt{5}}{\sqrt{9}}=\frac{\sqrt{5}}{3}$

$\sqrt{\frac{5}{8}}=\frac{\sqrt{5}}{\sqrt{2\times4}}=\frac{\sqrt{5}}{2\sqrt{2}}=\frac{\sqrt{5}\times\sqrt{2}}{2\sqrt{2}\times\sqrt{2}}=\frac{\sqrt{10}}{4}$

### Square root

A square root is a number that can be multiplied by itself to give us the value under the radical symbol (also referred to as the radix).

![alt](https://www.math.net/img/a/algebra/radical/square-root/sqrt.svg)

In the figure above, z is the square root of x.

We can also write this as "z raised to the power of 2 is equal to x" as follows:  
$z^2=x$

Example:
Solve: $2x^2 \times -8 = 0$  
$2(x^2-4)=0$  
$x^2-4=0$  
$\sqrt{x^2}=\sqrt{4}$  
$x=\pm\sqrt{4}=\pm2$

## Solving equations

### Completing the square

see also [Perfect Square Trinomial](#perfect-square-trinomial)

Generally, the goal behind completing the square is to create a perfect square trinomial from a quadratic.  
A perfect square trinomial is a trinomial that will factor into the square of a binomial.

The square of $x + n$ is $x^2 + 2nx + n^2$. As you can see, the coefficient of x is $2n$.  
For a quadratic of the form $x^2 + bx + c$, the coefficent of $x$ is already $b$, so we only need to figure out the value of the constant $c$. 

If $2n = b$, then $n = \frac{b}{2}$. Therefore, the binomial used to complete the square is: $x \pm \frac{b}{2}$  
If we square this binomial, the perfect square trinomial needed to complete the square will equal:

---

$(a+b)^2=a^2+2ab+b^2$

$(3+4)^2$  
$=3^2+2\times3\times4+4^2$, ALSO $3^2+(2\times3)\times4+4^2$, ALSO $3^2+(2\times4)\times3+4^2$    
$=9+24+16$

<br/>

$2b=k$, $b=\frac{k}{2}$; $2\times4=8$, $4=\frac{8}{2}$

---

$(x+\frac{b}{2})^2=x^2+bx+(\frac{b}{2})^2$  
OR  
$(x-\frac{b}{2})^2=x^2-bx+(\frac{b}{2})^2$  

<br/>

1 Write the given equation in the standard form of the quadratic equation:  
$ax^2+bx+c=0$

Example  

$2x^2=7x-6$  
$2x^2-7x+6=0$

<br/>

2 *Factor out* and divide both sides by the coefficient of $x^2$ if it does not already equal 1:

$2x^2-7x+6=0$

$2(x^2-\frac{7}{2}x+3)=0$

$x^2-\frac{7}{2}x+3=0$

Note: Dividing both sides by 2 cancels out 2 on the left side of the equation. On the right, $\frac{0}{2}=0$.  

<br/>

3 Move the constant to the other side of the equation.

$x^2-\frac{7}{2}x=-3$

<br/>

4 Add $(\frac{b}{2})^2$ to both sides of the equation (to keep them equivalent):

$x^2-\frac{-7}{2}x=-3$

$b=\frac{-7}{2}; \quad \frac{b}{2}=-\frac{7}{4}; \quad (\frac{b}{2})^2=(-\frac{7}{4})^2$

$x^2-\frac{7}{2}x+(\frac{-7}{4})^2=-3+(\frac{-7}{4})^2$

$x^2-\frac{7}{2}x+(\frac{-7}{4})^2=-3+\frac{49}{16}=\frac{-3}{1}+\frac{49}{16}=\frac{-48}{16}+\frac{49}{16}$

$x^2-\frac{7}{2}x+(\frac{-7}{4})^2=\frac{1}{16}$

Factor the side with $x^2+bx+(\frac{b}{2})^2 \quad to \quad (x+\frac{b}{2})^2$

$x^2-\frac{7}{2}x+(\frac{-7}{4})^2=\frac{1}{16}$

$(x-\frac{7}{4})^2=\frac{1}{16}$

Solve for x:

$\sqrt{(x-\frac{7}{4})^2}=\sqrt{\frac{1}{16}}$

$x-\frac{7}{4}=\pm\frac{1}{4}$

$x=\frac{7}{4}\pm\frac{1}{4}$

$x=2 \quad or \quad x=\frac{3}{2}$


### Discriminant

$b^2-4ac$

If the discriminant is less than 0, then the quadratic has no real solution.

### System of equations

#### Graphing method

by tools

#### Substitution method

replacing a variable in one equation with the equivalent of that variable

Variables with coefficients of 1 are the easiest to solve

Example

Get $y$ from a variable  
$3x + y = 31	‚Üí	y = -3x + 31$  

$2x - 5y = 15	‚Üí	-5y = 15 - 2x$  
$y=\frac{-2x+15}{-5}$

Next  
$y = -3x + 31$  
$2x - 5y = 15$  
$2x - 5(-3x + 31) = 15$

Then  
$2x - 5 (-3x + 31) = 15$  
$2x + 15x - 155 = 15$  
$17x = 170$  
$x = 10$  

The remaining variable  
$x = 10$  
$2(10) - 5y = 15$  
$-5y = -5$  
$y = 1$  

You can check your answers by plugging the x- and y-values  
$x = 10$  
$3x + y = 31$  
$3(10) + (1) = 31$  
$31 = 31$  

$y = 1$  
$2x - 5y = 15$  
$2(10) - 5(1) = 15$  
$15 = 15$  

#### Elimination method

Example

$
\begin{cases}
6x + 2y= 18\\
+5x + 4y= 22
\end{cases}
$


If uses $6x$, that would be difficult.  
$-\frac{5}{6} \times 6x=-5x$


$
\begin{cases}
-2(6x + 2y)= 18\\
+5x + 4y= 22
\end{cases}
$

$
\begin{cases}
-12x-4y=-36\\
+5x+4y= 22
\end{cases}
$  
$=\;\; -7x + 0=-14$

Then solve for x!  
$-7x= -14$  
$\quad\; x= 2$

Next, plug the value of x into one of the original equations to find the value of y.

$x= 2$  
$5(2)+ 4y= 22$  
$4y= 12$  
$y= 3$  

### Vertex form

#### Converting from standard form to vertex form

Example

$y = 3x^2 + 9x + 4$  
$y - 4 = 3x^2 + 9x$  
$y - 4 = 3(x^2 + 3x)$  
$y - 4 + 3(?) = 3(x^2 + 3x + ?)$  
$y - 4 + 3(\frac{9}{4}) = 3(x^2 + 3x + \frac{9}{4})$  
$y - \frac{16}{4}+\frac{27}{4}=3(x + \frac{3}{2})^2$  
$y = 3(x + \frac{3}{2})^2-\frac{11}{4}$  

---

Another way  

$y = 3x^2 + 9x + 4$  
$y=3(x^2+3x)+4$  


<mark style="">when no commom factors  
$y = 3x^2 + 10x + 4$  
$y=3(x^2+\frac{10}{3}x)+4$</mark>  

Get square number by coefficient 3  
$(\frac{3}{2})^2=\frac{9}{4}$

And make it keep identical  
**Add a square and substract a square when completing square**  

$x^2+3x=(x+\frac{3}{2})^2-\frac{9}{4}$  
$y=3((x+\frac{3}{2})^2-\frac{9}{4})+4$  
$y=3(x+\frac{3}{2})^2-3\times\frac{9}{4}+4$  
$y=3(x+\frac{3}{2})^2-\frac{27}{4}+4$  
$y=3(x+\frac{3}{2})^2-\frac{27}{4}+\frac{16}{4}$  
$y=3(x+\frac{3}{2})^2-\frac{11}{4}$  

## Exponents

### Exponents

https://www.math.net/exponent

An exponent is a number that tells us how many times the base it is attached to is used as a factor.

this context, and we can read $5^3$ as "five to the power of three," which works out to:

$5^3=5\times5\times5=125$

<br/>

In the case of a negative exponent,  
we can rearrange the expression by taking the reciprocal, then raising it to a positive exponent, as long as the base is a non-zero real number.

$5^{-3}=\frac{1}{5^3}=\frac{1}{125}$

<br/>

If an exponent is not an integer, and is positive, we take the $n^{th}$ root of the base, where n is the exponent.

$5^{\frac{1}{3}}=\sqrt[3]{5}$

#### Exponent properties

Any non-zero base raised to the power of 0 is 1.  
$123456789^0 = 1$

<br/>

$0^0$ is a special case that does not have a definite answer; it is most commonly said to equal 1, or is said to be undefined.

<br/>

0 taken to any power greater than 0 is 0. 0 taken to a negative exponent is undefined.  
$0^12345678=0$  
$0^{-5}=\frac{1}{0^5}=\frac{1}{0}=undefined$

<br/>

Any number taken to the power of 1 equals itself. 1 taken to the power of any number equals 1.  
$n^1 = n$  
$1^n = 1$

### Fractional exponents

### Negative exponents

A negative exponent is equal to the reciprocal of the base of the negative exponent raised to the positive power.  

$b^{-n}=\frac{1}{b^n}$


### Exponent rules

### Power

#### Basic power properties

If the power is a positive integer, then the power tells us how many times to multiply the base by itself.  
$5^2=5\times5=25$

<br/>

If the power is a negative integer, -n, and b is a non-zero real number, we take the reciprocal of the base raised to the power of n.  
$b{-n}=\frac{1}{b^n}$  
$5^{-2}=\frac{1}{5^2}=\frac{1}{25}=0.04$

<br/>

Anything raised to the power of 0 is 1. $0^0$ is a special case that is either considered 1 or undefined.  
$136^0=1$

<br/>

If the power is a fraction, we take the $n^th$ root of the base, where n is the number in the denominator of the fraction.  
$2^{\frac{2}{3}}=\sqrt[3]{2^2}=\sqrt[3]{4}$


## Polynomial

https://www.math.net/polynomial

### binomial theorem

#### Summation

#### Combinations



## Logarithm

A logarithm is the inverse function of exponentiation.  
A logarithm tells us the power, y, that a base, b, needs to be raised to in order to equal x.  

This is written as:

$\log_b \; (x)=y$

Example

$10^3=1000; \quad so \quad \log_{10}(1000)=3$

### Log rules

#### Product rule

$log_b (mn) = log_b(m) + log_b(n)$

#### Quotient rule

$log_b(\frac{m}{n}) = log_b(m) - log_b(n)$

#### Power rule

$log_b(m^n) = n¬∑log_b(m)$

### ln

see also [natural-log](../math-gfg/logarithm.md#natural-log)

$ln(x)$ also $log_e(x)$

$\ln(e^x) = x$

### :pencil: e

#### 1\. The calculation is carried out through series expansion

$$e=\sum_ {n=0}^\infty \frac{1}{n!}$$

#### 2\. Calculate through limit definition

$$e = \lim_ {n \to \infty} (1+\frac{1}{n})^n	\approx 2.71828$$

$$e^x = \lim_ {n \to \infty} (1+\frac{x}{n})^n$$

#### 3\. Through continuous compound interest calculation

$$A = P(1 + \frac{r}{n})^n$$


- ùê¥ It's the final amount.
- ùëÉ It is the initial principal
- ùëü It is the annual interest rate (for example, 5% is 0.05).
- ùëõ It is the number of times compound interest is added (say compound interest once a year, ùëõ=1;) Compound interest per month, ùëõ=12)

---

When ùëõ=1 Ôºö
$A = P(1 + \frac{1}{1})^1 \approx 2$

When ùëõ=100 Ôºö
$A = P(1 + \frac{1}{100})^{100} \approx 2.70481$

When ùëõ=10000 Ôºö
$A = P(1 + \frac{1}{10000})^{10000} \approx 2.71815$

---

`var n = 100; Math.pow((1 +(1 / n)), n)`

Êé®ÂØºËøáÁ®ãÔºöËÆ°ÁÆó ùëí
ÂΩì ùëõ Ë∂ãÂêë‰∫éÊó†Á©∑Â§ßÊó∂Ôºå$(1 + \frac{1}{n})^n$ÁöÑÂÄº‰ºöË∂äÊù•Ë∂äÊé•Ëøë 2.71828...ÔºåËøôÂ∞±ÊòØÂ∏∏Êï∞ ùëí ÁöÑËøë‰ººÂÄº„ÄÇ

$$e = \lim_ {n \to \infty} (1+\frac{1}{n})^n	\approx 2.71828$$

## Factoring

### How to factor

#### Finding common factors

#### FOIL method

FOIL is a method for factoring that involves using the FOIL method of binomial expansion, backwards.

Set up a product of binomials. 

1. Write 2 empty parentheses that will be filled with 2 binomials that are equivalent to the original equation.
2. Write values for the first term in each binomial such that the product of the values <u>is equal to the first term</u> of the expression being factored.
3. Find a product of two values that <u>is equal to the third term</u> in the expression being factored, <u>that when added, equals the coefficient of the second term</u> in the equation. Write each value as the second term in each binomial with the appropriate sign.

**Example**  

Factor $x^2+3x-28$:  

1.	$(‚ÄÉ‚ÄÉ)  (‚ÄÉ‚ÄÉ)$
2.	$(x‚ÄÇ‚ÄÉ)  (x‚ÄÇ‚ÄÉ)$
3.	$(x + 7) (x - 4)$


<br/>
<br/>

:pencil: **Example**  
$(x+2)(x+3)$  
FÔºàFirstÔºâÔºö $x √ó x = x¬≤$  
OÔºàOuterÔºâÔºö $x √ó 3 = 3x$  
IÔºàInnerÔºâÔºö $2 √ó x = 2x$  
LÔºàLastÔºâÔºö $2 √ó 3 = 6$  

then  
$x^2+3x+2x+6=x^2+5x+6$

#### :pencil: Cross Factorization Method

$x^2+5x+6$

Find intergers of $p, q$ then: $p+q=5,p√óq=6$  
$p=2,q=3$

so

$x^2+5x+6=(x+2)(x+3)$

### Factoring polynomials

### Prime factors

A prime factor is a factor that is a prime quantity, meaning that it can only be formed as the product of 1 and itself. For example, $3 √ó 7 = 21$. In this problem, $3$ and $7$ are prime factors,

### Prime factorization

#### Trial division

#### Factor tree

## Complex numbers

### Imaginary numbers

## Sequence

### Arithmetic sequence

the difference between each term in the following sequence is 3

2, 5, 8, 11, 14, 17, 20 ...

$a_n = a_1 + (n - 1)d$  
$a_n = 2 + 3n - 3 = 3n - 1$

#### Arithmetic sequence vs arithmetic series

An arithmetic series is the sum of a finite part of an arithmetic sequence.

$$\frac{n}{2}(2a_1+(n-1)d)$$

**Example**  
Find the sum of the first 7 terms in the arithmetic sequence 1, 7, 13, 19, 25, ...


the sequence is 6  
The first 7 terms are:  1, 7, 13, 19, 25, 31, 37

The sum of these terms is:  
$\frac{n}{2}(2a_1+(n-1)d)$  

$\quad\frac{7}{2}(2a_1+(7-1)6)$  
$=\frac{7}{2}(2+36)$  
$=133$



### Geometric sequence

each subsequent term after the first term is determined by multiplying the previous term by a constant (not 1), which is referred to as the common ratio.


To determine the nth term of the sequence, the following formula can be used:  
$$a_n=ar^{n-1}$$

where $a_n$ is the nth term in the sequence,  
$r$ is the common ratio,  
and $a$ is the value of the first term.

<br/>

**Example**  
Find the 12th term of the geometric series: 1, 3, 9, 27, 81, ...

$a_n = ar^{n-1} = 1(3^{(12 - 1)}) = 3^11 = 177,147$

#### Geometric sequence vs geometric series

$$\frac{a(1-r^n)}{1-r}$$

**Example**  
Find the sum of the first 12 terms in the geometric series: 1, 3, 9, 27, 81,...

$\frac{a(1-r^n)}{1-r} = \frac{1(1-3^12)}{1-3} = 265,720$

### Summation

#### Sigma notation

For example, the sum of the integers 1, 2, 3, 4, and 5 can be expressed in sigma notation as:  
$$\sum_{n=1}^5 n$$

Expanding the above summation:  
$$\sum_{n=1}^5 n = 1+2+3+4+5=15$$

Examples:  

$$\sum_{n=1}^6 n^2$$
$$\sum_{n=1}^6 n^2 = 1^2+2^2 ... = 91$$

---

$$\sum_{n=1}^3 2n+1$$
$$\sum_{n=1}^3 2n+1 = (2¬∑1+1) + (2¬∑2+1) + (2¬∑3+1) = 15 $$

## Inequality

### Properties of inequalities--inside

### Inequality symbols

## Variable

In algebra, a variable is usually a letter or other symbol that stands for a number or quantity that may vary.

### Direct variation


### Inverse variation


### Constant of proportionality


### Dependent variable

Real world examples of a dependent variable include:  
the height of a plant as a function of the amount that it is watered, where the amount it is watered is the independent variable;  

the score on a test a student achieves as a function of the amount that they studied, where the independent variable is the amount of time that they studied;  

the amount of money you earn as a function of the amount of time worked, where the amount of time worked is the independent variable.

## Function

A function is a relation between two sets in which each member of the first set is paired with one, and only one, member of the second set.

A function rule is a rule that explains the relationship between two sets.

[Algebra-Function](./Algebra-Function.md)

## Linear equations

### Intro

#### Forms of linear equations

**Slope-intercept form**  

$y = mx + b$

where m is the slope, and b is the y-intercept.

**Point-slope form**  

it is based on some point on the line.

$y - y_1 = m(x - x_1)$

where $(x_1, y_1)$ represent a point on the line, and m is the slope. 

**Standard form**  

$Ax + By = C$

### Slope

Slope is a value that describes the steepness and direction of a line. The slope formula is as follows:

$$m = \frac{change\;in\;y}{change\;in\;x} = \frac{rise}{run} = \frac{y_2-y_1}{x_2-x_1}$$

#### Rise over run


<div align="center">

![alt](https://www.math.net/img/a/algebra/linear-equations/slope/ror.png)

</div>

**Example**  
Given the following points:

(-2, 3) and (4, 1)

$\frac{y_2-y_1}{x_2-x_1} = \frac{(1)-(3)}{(4)-(-2)} = \frac{-2}{6} = \frac{-1}{3}$

#### Positive slope

Slope also indicates the direction of a line.  
A line with a positive slope, said to be increasing, runs upwards from left to right.

<div align="center">

![alt](https://www.math.net/img/a/algebra/linear-equations/slope/sl1.png)

</div>

$$y=\frac{1}{2}x-3$$

#### Negative slope

A line with a negative slope, said to be decreasing, runs downwards from left to right.

<div align="center">

![alt](https://www.math.net/img/a/algebra/linear-equations/slope/sl2.png)

</div>

$$y=-5x+2$$

#### Horizontal line slope

A horizontal line has a slope of zero because y does not change:

<div align="center">

![alt](https://www.math.net/img/a/algebra/linear-equations/slope/sl3.png)

</div>

$$y=2$$

#### Vertical line slope

A vertical line has an undefined slope because you cannot divide by zero (x does not change).

<div align="center">

![alt](https://www.math.net/img/a/algebra/linear-equations/slope/sl4.png)

</div>

$$x = 3$$

#### Parallel line slope

$y = 2x + 3$ and $y = 2x - 4$ both have a slope of 2, so they are parallel, as shown below:

<div align="center">

![alt](https://www.math.net/img/a/algebra/linear-equations/slope/parallel.png)

</div>

#### Perpendicular line slope

Perpendicular lines have slopes that are "opposite reciprocals" of each other.  
In this context, "opposite" refers to the change in sign from + to - or vice versa. "Reciprocal" refers to flipping the numerator and denominator of the value.


$-3x - 2$ has a slope of -3, and $y = \frac{1}{3}x + 1$ has a slope of $\frac{1}{3}$. -3 and $\frac{1}{3}$ are opposite reciprocals, so the equations are perpendicular:

<div align="center">

![alt](https://www.math.net/img/a/algebra/linear-equations/slope/perpendicular.png)

</div>

### Intercept

The x-intercept is the point at which a line crosses the x-axis and the y-intercept is the point at which a line crosses the y-axis. 

<div align="center">

![alt](https://www.math.net/img/a/algebra/linear-equations/intercept/int.svg)

</div>

Given the equation of a line, it is possible to find the x and y-intercepts by plugging in 0 for either x or y.  
Plugging 0 in for x then solving for y yields the y-intercept.  
Plugging 0 in for y then solving for x yields the x-intercept.

**Example**  
Find the x and y-intercepts of line $2x - 8y = 16$.

Substituting 0 in for x:  
$2(0) - 8y = 16$  
$-8y = 16$  
$y = -2$  

The y-intercept is at (0, -2).

<br/>

Substituting 0 in for y:  
$2x - 8(0) = 16$  
$2x = 16$  
$x = 8$  

The x-intercept is at (8, 0).

Since we know two points on the line (the intercepts) we can plot the line, as shown below.

<div align="center">

![alt](https://www.math.net/img/a/algebra/linear-equations/intercept/line.svg)

</div>


### Slope formula

The slope of a line, "m" in the equation for a line of the form $y = mx + b$, can be found using the slope formula as long as at least two points on the line are known.

$$Slope = \frac{change in y}{change in x} = \frac{y_2 - y_1}{x_2 - x_1}$$


**Example**  
Given two points, (1, 3) and (4, 7), we can plug them into the formula to find the slope:  
$Slope = \frac{7-3}{4-1} = \frac{4}{3}$

The slope is $\frac{4}{3}$  which means that for every increase of 4 units in y, there is an increase of 3 units in x.   
Change in y is sometimes referred to as "rise" while change in x is referred to as "run."

<br/>

Note that even though we chose to use (4, 7) as x2 and y2, we could've also used it as x1 and y1 to achieve the same result:  
$Slope = \frac{3-7}{1-4} = \frac{-4}{-3} = \frac{4}{3}$

### Slope intercept form

$y = mx + b$

m is the slope, and b is the y-intercept. 

**Example**  
Given m = 3 and the point (3, 5), find b, and write the equation of the line in slope-intercept form.

$y = mx + b$  
$(5) = (3)(3) + b$  
$b = 5 - 9 = -4$  
$y = 3x - 4$  

![alt](https://www.math.net/img/a/algebra/linear-equations/slope-intercept-form/sif.png)


#### How to find the slope and the y-intercept

Given at least two points on a line, the slope of the line can be found using the slope formula:

$$\frac{change in y}{change in x} = \frac{rise}{run} = \frac{y_2-y_1}{x_2-x_1}$$

<br/>
For example, given the that (1, 5) and (-2, 7) are points on the same line, the slope of the line can be found as follows:

$$m = \frac{7-5}{-2-1} = -\frac{2}{3}$$

#### Other forms of linear equations

##### Point-slope form

$y - y_1 = m(x - x_1)$

##### Standard form

$Ax + By = C$

#### Converting between different forms

##### Standard to slope-intercept form

Converting from standard form to slope-intercept form involves manipulating an equation in standard form so as to isolate y on one side of the equation such that the coefficient on the y is 1.

**Example**  
Convert $2x - 5y + 6 = 0$ to slope-intercept form.

$5y = 2x + 6$

$y = \frac{2x}{5} + \frac{6}{5}$

The slope is therefore $\frac{2}{5}$, and the y-intercept is at $(0, \frac{6}{5})$.


:pencil: Note:  
$2x - 5y + 6 = 0$  

$‚àí5y=‚àí2x‚àí6$  
$y = \frac{-2x-6}{-5}$  
$y = \frac{2}{5}x + \frac{6}{5}$  


##### Point-slope to slope-intercept form

Converting from point-slope form to slope-intercept form is relatively simple since both already include a slope, so all we need to do is convert the equation such that we can read off the y-intercept, rather than some other point on the line.

**Example**  
Convert $y - 7 = \frac{1}{2}(x - 4)$ to slope-intercept form.

$y = \frac{1}{2}x - \frac{4}{2} + 7$

$y = \frac{1}{2}x + 5$

### Point slope form

$y - y_1 = m(x - x_1)$

where m is the slope of the line,  
(x1, y1) is a point on the line,  
and x and y are variables representing other points on the line.

Notice that point-slope form is more or less a rearranged form of the slope formula, $y = mx + b$:

$$m = \frac{y_2-y_1}{x_2-x_1}$$
$$(x_2-x_1)m = \frac{y_2-y_1}{x_2-x_1}(x_2-x_1)$$
$$m(x_2-x_1) = (y_2-y_1)$$
$$(y_2-y_1) = m(x_2-x_1)$$

### Slope of a line

[Slope](#slope)

### Standard form


$$Ax + By = C$$

where A, B, and C are constants.

<br/>


**Find intercepts**  
Standard form is useful because the x- and y-intercepts of the line can be easily found by setting x or y equal to 0, then solving for the desired variable.

Doing so results in the general formulas for finding the x and y-intercept given a linear equation in standard form:

$$x-intercept = \frac{C}{A}$$

$$y-intercept = \frac{C}{B}$$


Example:  

$3x + 2y = 6$

$3x + 2(0) = 6$  
$3x = 6$  
$x = 2$  

x-intercept at (2, 0)

<br/>

$3(0) + 2y = 6$  
$2y = 6$  
$y = 3$  

y-intercept at (0, 3)

<div align="center">

![alt](https://www.math.net/img/a/algebra/linear-equations/standard-form/stf.png)

</div>


#### Converting to standard form

Converting from point-slope or slope-intercept form to standard form involves moving all the variables to one side of the equation, moving the constant to the other side,  
then manipulating the equation as necessary such that the coefficients of the terms of the equation are integers.


**Examples**  
Convert the following linear equations to standard form.

1\. $y = -\frac{3}{4}x + 2$:

$\frac{3}{4}x + y = 2$  
$3x + 4y = 8$


2\. $y - 2 = \frac{3}{4}(x - 8)$:

$y - 2 = \frac{3}{4}x - 6$  
$-\frac{3}{4}x + y = 4$  
$-3x + 4y = 16$


### Midpoint formula

Given a line segment with endpoints A and B, the midpoint is the point located exactly between A and B, meaning that it is the same distance from A and B, as in the figure below.

<div align='center'>

![alt](https://www.math.net/img/a/algebra/linear-equations/midpoint-formula/mp.svg)

</div>


The midpoint formula can be used when two points on a graph in the coordinate plane are known.  
Given two points $(x1, y1)$ and $(x2, y2)$, their midpoint $M$ is:

$$M = (\frac{x1+x2}{2}, \frac{y1+y2}{2})$$

<br/>

Notice that the midpoint formula involves taking an average of the x- and y-values of two coordinates. 

**Example**  

$(x,y) \rightarrow (-3, 5) \qquad (x1,y1) \rightarrow (-1, 3)$  

<br/>

$M = (\frac{x1+x2}{2},\frac{y1+y2}{2})$  
$=(\frac{(-3)+(-1)}{2}, \frac{(-5)+(3)}{2})$  
$=(\frac{-4}{2}, \frac{-2}{2})$  
$=(-2,-1)$



<div align='center'>

Midpoint at (-2, -1)

![alt](https://www.math.net/img/a/algebra/linear-equations/midpoint-formula/mf.png)

</div>

$\hat{y}=b_0+b_1x$